Let the handlers infer the effect stack #116
The shape and position function arguments in the
generalized effect smart constructors are now
explicit. This means that we can define an effectful
program that takes Shape and Pos as arguments
and then handle the program by letting the handlers
infer the appropriate effect stack.

The handler tests have also been adjusted so that
no fixed effect stack is used for effectful programs
like coin or traceOne.

base/Free/Instance/ND.v
@@ -23,12 +23,12 @@ Module ND.
   Module Import Monad.
     Definition ND (A : Type) : Type := Free Shape Pos A.
 
-    Definition Fail {A : Type} {Shape' : Type} {Pos' : Shape' -> Type} 
+    Definition Fail {A : Type} (Shape' : Type) (Pos' : Shape' -> Type) 
       `{Injectable Shape Pos Shape' Pos'} 
       : Free Shape' Pos' A :=
       impure (injS sfail) (fun p => (fun (x : Void) => match x with end) (injP p)).
 
-    Definition Choice {A : Type} {Shape' : Type} {Pos' : Shape' -> Type} 
+    Definition Choice {A : Type} (Shape' : Type) (Pos' : Shape' -> Type) 
     `{Injectable Shape Pos Shape' Pos'} mid l r
     : Free Shape' Pos' A := 
        let s := injS (schoice mid) 
@@ -36,7 +36,7 @@ Module ND.
 
     (* Curry notation for the choice operator. 
        The ID is set by the sharing handler. *)
-    Notation "x ? y" := (Choice None x y) (at level 80).
+    Notation "x ? y" := (Choice _ _ None x y) (at level 80).
  End Monad.
 
   (* Handlers for non-determinism and call-time choice. *)
@@ -96,8 +96,8 @@ Module ND.
           | impure (inr (inl (ND.schoice id))) pf =>
              let l := nameChoices (next + 1) scope scopes (pf true) in
              let r := nameChoices (next + 1) scope scopes (pf false) in
-             Choice (Some (tripl scope next)) l r
-          | impure (inr (inl ND.sfail)) _ => Fail
+             Choice (SChoice Shape') (PChoice Pos') (Some (tripl scope next)) l r
+          | impure (inr (inl ND.sfail)) _ => Fail (SChoice Shape') (PChoice Pos')
           | impure (inr (inr s)) pf =>
              impure (inr s) (fun p => nameChoices next scope scopes (pf p))
           end
@@ -118,8 +118,8 @@ Module ND.
 
   (* Partial instance for the non-determinism effect. *)
   Instance Partial : Partial Shape Pos := {
-      undefined := fun {A : Type}                => Fail;
-      error     := fun {A : Type} (msg : string) => Fail
+      undefined := fun {A : Type}                => Fail Shape Pos;
+      error     := fun {A : Type} (msg : string) => Fail Shape Pos
     }.
 End ND.
 
