base/Free/Test.v
@@ -11,94 +11,91 @@ From Base Require Import Free.Malias.
 
 From Base Require Import Prelude.Bool.
 From Base Require Import Prelude.Integer.
+From Base Require Import Prelude.List.
+From Base Require Import Prelude.Pair.
 
 From Base Require Import Free.Util.Search.
 
 Require Import Lists.List.
 Import List.ListNotations.
 
-(* Synonym for cbneed for better readability. *)
-Definition share {A : Type} 
-                 {Shape : Type} 
-                 {Pos : Shape -> Type}
-                 `{i : Injectable Share.Shape Share.Pos Shape Pos} 
-                 (x : Free Shape Pos A) 
-:= @cbneed A Shape Pos i x.
+
+
+Definition share {A : Type} {Shape : Type} {Pos : Shape -> Type}
+  `{i : Injectable Share.Shape Share.Pos Shape Pos} x := @cbneed A Shape Pos i x.
+
+(* Some synonyms for programs containing non-determinism for convenience. *)
+Definition NDShape := (Comb.Shape Share.Shape (Comb.Shape ND.Shape Identity.Shape)). 
+Definition NDPos := (Comb.Pos Share.Pos (Comb.Pos ND.Pos Identity.Pos)).
+Definition NDProg (A : Type) := Free NDShape NDPos A.
+
+(* Some synonyms for programs containing tracing for convenience. *)
+Definition TraceShape := (Comb.Shape Share.Shape (Comb.Shape Trace.Shape Identity.Shape)). 
+Definition TracePos := (Comb.Pos Share.Pos (Comb.Pos Trace.Pos Identity.Pos)).
+Definition TraceProg (A : Type) := Free TraceShape TracePos A.
+
+(* Synonyms for programs containing non-determinism and partiality. *)
+Definition NDMShape := Comb.Shape Maybe.Shape NDShape.
+Definition NDMPos := Comb.Pos Maybe.Pos NDPos.
+Definition NDMProg (A : Type) := Free NDMShape NDMPos A.
+
+(* Synonyms for programs containing tracing and partiality. *)
+Definition TraceMShape := Comb.Shape Maybe.Shape TraceShape.
+Definition TraceMPos := Comb.Pos Maybe.Pos TracePos.
+Definition TraceMProg (A : Type) := Free TraceMShape TraceMPos A.
 
 (* Shortcut to evaluate a non-deterministic program to a result list.
    list. *)
-Definition evalND {A : Type} p
-:= @collectVals A (run (runChoice (runNDSharing (0,0) p))).
+Definition evalND {A : Type} (p : NDProg A) 
+:= collectVals (run (runChoice (runNDSharing (0,0) p))).
 
 (* Shortcut to evaluate a traced program to a result and a list of logged 
    messages. *)
-Definition evalTracing {A : Type} p 
-:= @collectMessages A (run (runTracing (runTraceSharing (0,0) p))).
-
-Check evalTracing.
+Definition evalTracing {A : Type} (p : TraceProg A) 
+:= collectMessages (run (runTracing (runTraceSharing (0,0) p))).
 
 (* Shortcut to evaluate a non-deterministic partial program to a result 
    list. *)
-Definition evalNDM {A : Type} p
-:= @collectVals (option A) (run (runChoice (runNDSharing (0,0) (runMaybe p)))).
+Definition evalNDM {A : Type} (p : NDMProg A) 
+:= collectVals (run (runChoice (runNDSharing (0,0) (runMaybe p)))).
 
 (* Shortcut to evaluate a traced partial program to a result and a list 
    of logged messages. *)
-Definition evalTraceM {A : Type} p
-:= @collectMessages (option A) (run (runTracing (runTraceSharing (0,0) (runMaybe p)))).
+Definition evalTraceM {A : Type} (p : TraceMProg A)
+:= collectMessages (run (runTracing (runTraceSharing (0,0) (runMaybe p)))).
 
 (* Non-deterministic integer. *)
-Definition coin (Shape : Type) (Pos : Shape -> Type)
-                `{Injectable ND.Shape ND.Pos Shape Pos}
+Definition coin : NDProg (Integer NDShape NDPos)
 := pure 0%Z ? pure 1%Z.
-Arguments coin {_} {_} {_}.
-
 
 (* Non-deterministic boolean value. *)
-Definition coinB (Shape : Type) (Pos : Shape -> Type)
-                 `{Injectable ND.Shape ND.Pos Shape Pos}
+Definition coinB : NDProg (Bool NDShape NDPos)
  := True_ _ _ ? False_ _ _.
-Arguments coinB {_} {_} {_}.
 
 (* Non-deterministic partial integer. *)
-Definition coinM (Shape : Type) (Pos : Shape -> Type)
-                 `{Injectable ND.Shape ND.Pos Shape Pos}
-                 `{Injectable Maybe.Shape Maybe.Pos Shape Pos}
-:= (Nothing_inj _ _) ? (Just_inj _ _ 1%Z).
-Arguments coinM {_} {_} {_} {_}.
+Definition coinM : NDMProg (Integer NDMShape NDMPos)
+:= Nothing_inj ? Just_inj 1%Z.
 
 (* Traced integer. *)
-Definition traceOne (Shape : Type) (Pos : Shape -> Type)
-                    `{Injectable Trace.Shape Trace.Pos Shape Pos}
-:= trace "One" (pure 1%Z).
-Arguments traceOne {_} {_} {_}.
+Definition traceOne : TraceProg (Integer TraceShape TracePos) 
+:= trace "Log!" (pure 1%Z).
 
 (* Traced boolean values. *)
-Definition traceTrue (Shape : Type) (Pos : Shape -> Type)
-                     `{Injectable Trace.Shape Trace.Pos Shape Pos}
+Definition traceTrue : TraceProg (Bool TraceShape TracePos)
 := trace "True" (True_ _ _).
-Arguments traceTrue {_} {_} {_}.
-Definition traceFalse (Shape : Type) (Pos : Shape -> Type)
-                      `{Injectable Trace.Shape Trace.Pos Shape Pos}
+Definition traceFalse : TraceProg (Bool TraceShape TracePos)
 := trace "False" (False_ _ _).
-Arguments traceFalse {_} {_} {_}.
 
 (* Traced Maybe values *)
-Definition traceNothing (Shape : Type) (Pos : Shape -> Type)
-                        `{Injectable Trace.Shape Trace.Pos Shape Pos}
-                        `{Injectable Maybe.Shape Maybe.Pos Shape Pos}
-:= trace "Nothing" (@Nothing_inj (Integer Shape Pos) _ _ _).
-Arguments traceNothing {_} {_} {_} {_}.
-Definition traceJust (Shape : Type) (Pos : Shape -> Type)
-                     `{Injectable Trace.Shape Trace.Pos Shape Pos}
-                     `{Injectable Maybe.Shape Maybe.Pos Shape Pos}
-:= trace "Just 1" (Just_inj _ _ 1%Z).
-Arguments traceJust {_} {_} {_} {_}.
+Definition traceNothing : TraceMProg (Integer TraceMShape TraceMPos)
+:= trace "Nothing" Nothing_inj.
+Definition traceJust : TraceMProg (Integer TraceMShape TraceMPos)
+:= trace "Just 1" (Just_inj 1%Z).
 
 
-(* ---------------------- Test cases without sharing ----------------------- *)
+(* ------------ Examples ------------- *)
 
-(* This function applies the given binary function to the given argument
+(* This function applies the given binary function to the given argument 
    twice and does not share the argument. *)
 Definition double {Shape : Type}
                   {Pos : Shape -> Type}
@@ -121,12 +118,12 @@ Example exAddNoSharingND : evalND (double addInteger coin) = [0%Z;1%Z;1%Z;2%Z].
 Proof. constructor. Qed.
 
 (*
-trace "One" 1 + trace "One" 1
+trace "Log!" 1 + trace "Log!" 1
 => The message should be logged twice and the result should be 2.
 *)
 Example exAddNoSharingTrace 
 : evalTracing (double addInteger traceOne) 
-  = (2%Z,["One"%string;"One"%string]).
+  = (2%Z,["Log!"%string;"Log!"%string]).
 Proof. constructor. Qed.
 
 (*
@@ -145,7 +142,7 @@ Proof. constructor. Qed.
    message should be logged only once.
 *)
 Example exOrTrueTracingNoSharing 
- : evalTracing (orBool _ _ traceTrue traceTrue) 
+ : evalTracing (orBool TraceShape TracePos traceTrue traceTrue) 
    = (true,["True"%string]).
 Proof. constructor. Qed.
 
@@ -155,7 +152,7 @@ Proof. constructor. Qed.
    should be logged twice.
 *)
 Example exOrFalseTracingNoSharing 
- : evalTracing (orBool _ _ traceFalse traceFalse) 
+ : evalTracing (orBool TraceShape TracePos traceFalse traceFalse) 
    = (false,["False"%string;"False"%string]).
 Proof. constructor. Qed.
 
@@ -165,7 +162,7 @@ Proof. constructor. Qed.
    should be logged.
 *)
 Example exOrMixedTracingNoSharing
- : evalTracing (orBool _ _ traceFalse traceTrue) 
+ : evalTracing (orBool TraceShape TracePos traceFalse traceTrue) 
    = (true,["False"%string;"True"%string]).
 Proof. constructor. Qed.
 
@@ -199,8 +196,7 @@ Example exTraceJustNoSharing
    = (Some 2%Z,["Just 1"%string;"Just 1"%string]).
 Proof. constructor. Qed.
 
-
-(* --------------------- Test cases for simple sharing --------------------- *)
+(* Simple sharing *) 
 
 (* let sx = fx in f sx sx *)
 Definition doubleShared {Shape : Type}
@@ -225,12 +221,12 @@ Example exAddSharingND : evalND (doubleShared addInteger coin) = [0%Z;2%Z].
 Proof. constructor. Qed.
 
 (*
-let sx = trace "One" 1
+let sx = trace "Log!" 1
 in sx + sx
 => The message should be logged once and the result should be 2.
 *)
 Example exAddSharingTrace 
- : evalTracing (doubleShared addInteger traceOne) = (2%Z,["One"%string]).
+ : evalTracing (doubleShared addInteger traceOne) = (2%Z,["Log!"%string]).
 Proof. constructor. Qed.
 
 (*
@@ -267,7 +263,7 @@ Proof. constructor. Qed.
    Therefore, sharing should make no difference here. *)
 Example exOrMixedTraceSharing
  : evalTracing (share traceFalse >>= fun sx => 
-                orBool _ _ sx traceTrue)
+                orBool TraceShape TracePos sx traceTrue)
    = (true,["False"%string;"True"%string]).
 Proof. constructor. Qed.
 
@@ -301,7 +297,8 @@ Example exTraceJustSharing
  : evalTraceM (doubleShared addInteger traceJust) = (Some 2%Z,["Just 1"%string]).
 Proof. constructor. Qed.
 
-(* --------------------- Test cases for nested sharing --------------------- *)
+
+(* Nested sharing *)
 
 (* let sx = fx 
        sy = f sx sx
@@ -331,14 +328,14 @@ Example exAddNestedSharingND : evalND (doubleSharedNested addInteger coin)
 Proof. constructor. Qed.
 
 (* 
-let sx = trace "One" 1
+let sx = trace "Log!" 1
     sy = sx + sx 
 in sy + sy 
 => The message should only be logged once and the result should be 4. 
 *)
 Example exAddNestedSharingTrace 
  : evalTracing (doubleSharedNested addInteger traceOne) 
-   = (4%Z,["One"%string]).
+   = (4%Z,["Log!"%string]).
 Proof. constructor. Qed.
 
 (*
@@ -409,15 +406,15 @@ Example exAddClashSharingND
 Proof. constructor. Qed.
 
 (*
-let sx = trace "One" 1
+let sx = trace "Log!" 1
     sy = sx + sx
-    sz = trace "One" 1
+    sz = trace "Log!" 1
 in sy + sz
 => The message should be logged twice and the result should be 3.
 *)
 Example exAddClashSharingTracing
  : evalTracing (doubleSharedClash addInteger traceOne traceOne) 
-   = (3%Z,["One"%string;"One"%string]).
+   = (3%Z,["Log!"%string;"Log!"%string]).
 Proof. constructor. Qed.
 
 (*
@@ -504,8 +501,8 @@ Proof. constructor. Qed.
 
 (*
 let sx = 1
-    sy = sx + trace "One" 1
-    sz = sy + trace "One" 1
+    sy = sx + trace "Log!" 1
+    sz = sy + trace "Log!" 1
 in sx + (sy + (sz + 1))
 => The message should be logged once for sy and once for sz, so it should be 
    logged twice in total. 
@@ -514,7 +511,7 @@ in sx + (sy + (sz + 1))
 *)
 Example exAddRecSharingTracing
  : evalTracing (doubleSharedRec addInteger traceOne traceOne 1%Z) 
-   = (7%Z,["One"%string;"One"%string]).
+   = (7%Z,["Log!"%string;"Log!"%string]).
 Proof. constructor. Qed.
 
 (*
@@ -534,47 +531,77 @@ let sx = false
     sy = sx or (true ? false)
     sz = sy or (true ? false)
 in sx or (sy or (sz or false))
-= false or ((false or true) or ((true or (true ? false)) or false)) ?
-  false or ((false or false) or ((false or (true ? false)) or false))
-= (false or true) or ((true or (true ? false)) or false) ?
-  (false or false) or ((false or (true ? false)) or false)
-= true ? 
-  (false or (true ? false)) or false
-= true ? 
-  (true ? false) or false
-= true ?
-  true or false ?
-  false or false
-= true ? true ? false
+= false or ((false or true)) ? 
 *)
-Example exOrRecSharingNDFalse
+Example exOrRecSharingNDTrue
  : evalND (doubleSharedRec orBool coinB coinB false)
-   = [true;true;false].
+   = [true].
 Proof. constructor. Qed.
 
-(* 
-let sx = false
-    sy = sx or (trace "True" true)
-    sz = sy or (trace "True" true)
-in sx or (sy or (sz or false))
-=> sy has the value true, so sz is not evaluated. The message should only 
-   be logged once and the result should be true.
-*)
-Example exOrRecTrueTracing
- : evalTracing (doubleSharedRec orBool traceTrue traceTrue false)
-   = (true,["True"%string]).
-Proof. constructor. Qed.
 
-(*
-let sx = false
-    sy = sx or (trace "False" false)
-    sz = sy or (trace "False" false)
-in sx or (sy or (sz or false))
-=> sy is shared, so its message should only be logged once. Additionally,
-   the message is logged once more when sz is evaluated. The result should
-   be false.
-*)
-Example exOrRecFalseTracing
- : evalTracing (doubleSharedRec orBool traceFalse traceFalse false)
-   = (false,["False"%string;"False"%string]).
-Proof. constructor. Qed.
+
+
+
+
+
+
+
+
+
+
+
+(* Deep sharing *)
+
+(* [0] ? [1] *)
+Definition NDList : NDProg (List NDShape NDPos (Integer NDShape NDPos))
+:= (Cons _ _ (pure 0%Z) (Nil _ _)) ? (Cons _ _ (pure 1%Z) (Nil _ _)).
+
+(* [0 ? 1] *)
+Definition coinList : NDProg (List NDShape NDPos (Integer NDShape NDPos))
+:= Cons _ _ coin (Nil _ _).
+
+(* trace "Log!" [1] *)
+Definition TraceList 
+ : TraceProg (List TraceShape TracePos (Integer TraceShape TracePos))
+:= trace "Log!" (Cons _ _ (pure 1%Z) (Nil _ _)).
+
+(* [trace "Log!" 1] *)
+Definition TraceInList 
+ : TraceProg (List TraceShape TracePos (Integer TraceShape TracePos))
+:= Cons _ _ traceOne (Nil _ _).
+
+Definition pairList {Shape : Type}
+               {Pos : Shape -> Type}
+               {A : Type}
+               (l : Free Shape Pos (List Shape Pos A))
+ : Free Shape Pos (Pair Shape Pos(List Shape Pos A) (List Shape Pos A))
+:= Pair_ Shape Pos l l.
+
+Definition pairListShared {Shape : Type}
+               {Pos : Shape -> Type}
+               {A : Type}
+               `{Injectable Share.Shape Share.Pos Shape Pos}
+               (l : Free Shape Pos (List Shape Pos A))
+ : Free Shape Pos (Pair Shape Pos(List Shape Pos A) (List Shape Pos A))
+:= share l >>= fun sl => Pair_ Shape Pos sl sl.
+
+(* Evaluated to [0,1] *)
+Compute evalND NDList.
+(* coin is not handled. *)
+Compute evalND coinList.
+
+(* Evaluated to [(1,["Log!"])].*)
+Compute evalTracing TraceList.
+(* Tracing inside the list is not handled. *)
+Compute evalTracing TraceInList.
+
+(* Needed: Normalization! *)
+
+(* Not handled *)
+Compute evalND (pairList NDList).
+Compute evalND (pairList coinList).
+
+(* Not handled *)
+Compute evalND (pairListShared NDList).
+Compute evalND (pairListShared coinList).
+
